WIP

demo/mutrec/MutrecHeader.v
@@ -88,3 +88,8 @@ Qed.
 (* Fixpoint sum (i: int): int := *)
 (*   i.(intval) *)
 (* . *)
+
+Require AST.
+
+Definition fg_sig: AST.signature := (AST.mksignature [AST.Tint] (Some AST.Tint) AST.cc_default).
+
